readme.md
@@ -1,0 +1,31 @@
+# Build
+
+Install [Isabelle 2017](https://isabelle.in.tum.de/), then run:
+
+	isabelle build -D .
+
+or:
+
+	isabelle build -D . -j 4 -o quick_and_dirty
+
+# Structure
+
+The following theory files are included:
+
+ - `prefix`: Lemmas about prefixes of lists.
+ - `repliss_sem`: This theory describes the distributed semantics used by Repliss.
+ - `execution_invariants`: This theory includes proof for invariants that hold for all executions.
+ - `commutativity`: This theory proves commutativity between certain actions in executions.
+ - `repliss_sem_single_invocation`: This theory describes the single-invocation semantics used for our proof approach.
+ - `execution_invariants_s`: This theory includes proof for invariants that hold for all single-invocation executions.
+ - `approach`: This theory includes the soundness proof of our proof approach.
+ - `single_invocation_correctness`: This theory includes techniques to prove that a program is correct in the single-invocation semantics.
+ - `invariant_simps`: This theory includes helpers for working with invariants.
+
+
+The lemmas and theorems from the paper can be found under the following names in the theories:
+
+- Lemma 5.1: `show_programCorrect_noTransactionInterleaving` in `commutativity`
+- Lemma 5.2: `convert_to_single_session_trace_invFail` in `approach`
+- Lemma 5.3: `show_correctness_via_single_session` in `approach`
+
